Semantic/CC/Syntax/Exp.lean
@@ -21,7 +21,7 @@ inductive Exp : Sig -> Type where
 | unit : Exp s
 | btrue : Exp s
 | bfalse : Exp s
-| cond : Exp s -> Exp s -> Exp s -> Exp s
+| cond : Var .var s -> Exp s -> Exp s -> Exp s
 
 /-- Applies a renaming to all bound variables in an expression. -/
 def Exp.rename : Exp s1 -> Rename s1 s2 -> Exp s2
@@ -38,7 +38,7 @@ def Exp.rename : Exp s1 -> Rename s1 s2 -> Exp s2
 | .unit, _ => .unit
 | .btrue, _ => .btrue
 | .bfalse, _ => .bfalse
-| .cond e1 e2 e3, f => .cond (e1.rename f) (e2.rename f) (e3.rename f)
+| .cond x e2 e3, f => .cond (x.rename f) (e2.rename f) (e3.rename f)
 
 /-- An expression is a value if it is an abstraction, pack, or unit. -/
 inductive Exp.IsVal : Exp s -> Prop where
@@ -134,6 +134,6 @@ inductive Exp.IsClosed : Exp s -> Prop where
 | unit : Exp.IsClosed .unit
 | btrue : Exp.IsClosed .btrue
 | bfalse : Exp.IsClosed .bfalse
-| cond : Exp.IsClosed e1 -> Exp.IsClosed e2 -> Exp.IsClosed e3 -> Exp.IsClosed (.cond e1 e2 e3)
+| cond : Var.IsClosed x -> Exp.IsClosed e2 -> Exp.IsClosed e3 -> Exp.IsClosed (.cond x e2 e3)
 
 end CC
