Semantic/CC/Semantics/SmallStep.lean
@@ -22,25 +22,18 @@ inductive Step : CapabilitySet -> Memory -> Exp {} -> Memory -> Exp {} -> Prop w
 | step_capply :
   m.lookup x = some (.val ⟨.cabs cs B e, hv, R⟩) ->
   Step C m (.capp (.free x) CS) m (e.subst (Subst.openCVar CS))
-| step_cond_true :
-  Step C m (.cond .btrue e1 e2) m e1
-| step_cond_false :
-  Step C m (.cond .bfalse e1 e2) m e2
 | step_cond_var_true :
   m.lookup x = some (.val ⟨.btrue, hv, R⟩) ->
-  Step C m (.cond (.var (.free x)) e1 e2) m e1
+  Step C m (.cond (.free x) e1 e2) m e1
 | step_cond_var_false :
   m.lookup x = some (.val ⟨.bfalse, hv, R⟩) ->
-  Step C m (.cond (.var (.free x)) e1 e2) m e2
+  Step C m (.cond (.free x) e1 e2) m e2
 | step_ctx_letin :
   Step C m e1 m' e1' ->
   Step C m (.letin e1 e2) m' (.letin e1' e2)
 | step_ctx_unpack :
   Step C m e1 m' e1' ->
   Step C m (.unpack e1 e2) m' (.unpack e1' e2)
-| step_ctx_cond :
-  Step C m e m' e' ->
-  Step C m (.cond e e1 e2) m' (.cond e' e1 e2)
 | step_rename :
   Step C m (.letin (.var (.free y)) e) m (e.subst (Subst.openVar (.free y)))
 | step_lift :
