Semantic/CC/TypeSystem/Core.lean
@@ -206,11 +206,11 @@ inductive HasType : CaptureSet s -> Ctx s -> Exp s -> Ty .exi s -> Prop where
   ----------------------------
   HasType {} Γ (.bfalse) (.typ (.capt {} .bool))
 | cond :
-  HasType C1 Γ e1 (.typ (.capt Cb .bool)) ->
+  HasType C1 Γ (.var x) (.typ (.capt Cb .bool)) ->
   HasType C2 Γ e2 T ->
   HasType C3 Γ e3 T ->
   ----------------------------
-  HasType (C1 ∪ C2 ∪ C3) Γ (.cond e1 e2 e3) T
+  HasType (C1 ∪ C2 ∪ C3) Γ (.cond x e2 e3) T
 | invoke :
   HasType (.var x) Γ (.var x) (.typ (.capt (.var x) .cap)) ->
   HasType (.var y) Γ (.var y) (.typ (.capt (.var y) .unit)) ->
